adapted to simplified T convention

thys/Priority_Queue_Braun/Priority_Queue_Braun.thy
@@ -263,18 +263,18 @@ apply(auto)
 done
 
 fun T_del_min :: "'a::linorder tree \<Rightarrow> nat" where
-"T_del_min Leaf = 1" |
-"T_del_min (Node Leaf x r) = 1" |
-"T_del_min (Node l x r) = 1 + (let (y,l') = del_left l in T_del_left l + T_sift_down r y l')"
+"T_del_min Leaf = 0" |
+"T_del_min (Node Leaf x r) = 0" |
+"T_del_min (Node l x r) = T_del_left l + (let (y,l') = del_left l in T_sift_down r y l')"
 
 lemma del_left_height: "\<lbrakk> del_left t = (x, t'); t \<noteq> \<langle>\<rangle> \<rbrakk> \<Longrightarrow> height t' \<le> height t"
 by(induction t arbitrary: x t' rule: del_left.induct) (auto split: prod.splits)
 
 lemma T_del_min_neq_Leaf: "l \<noteq> Leaf \<Longrightarrow>
-  T_del_min (Node l x r) = 1 + (let (y,l') = del_left l in T_del_left l + T_sift_down r y l')"
+  T_del_min (Node l x r) = T_del_left l + (let (y,l') = del_left l in T_sift_down r y l')"
 by (auto simp add: neq_Leaf_iff)
 
-lemma T_del_min: assumes "braun t" shows "T_del_min t \<le> 2*height t + 1"
+lemma T_del_min: assumes "braun t" shows "T_del_min t \<le> 2*height t"
 proof(cases t)
   case Leaf then show ?thesis by simp
 next
@@ -287,17 +287,17 @@ next
     obtain y l' where [simp]: "del_left l = (y,l')" by fastforce
     have 1: "height l' \<le> height l" by (simp add: \<open>l \<noteq> \<langle>\<rangle>\<close> del_left_height)
     have "braun \<langle>r, y, l'\<rangle>" using del_left_braun[of l y l'] \<open>l \<noteq> \<langle>\<rangle>\<close> assms del_left_size[of l] by auto
-    have "T_del_min t = 1 + T_del_left l + T_sift_down r y l'"
+    have "T_del_min t = T_del_left l + T_sift_down r y l'"
       using \<open>l \<noteq> Leaf\<close> by(simp add: T_del_min_neq_Leaf)
-    also have "\<dots> \<le> 1 + height l + T_sift_down r y l'"
+    also have "\<dots> \<le> height l + T_sift_down r y l'"
       using T_del_left_height[OF \<open>l \<noteq> Leaf\<close>] by linarith
-    also have "\<dots> \<le> 1 + height l + max(height r) (height l') + 1"
+    also have "\<dots> \<le> height l + max(height r) (height l') + 1"
       using T_sift_down_height[OF \<open>braun \<langle>r, y, l'\<rangle>\<close>, of y] by linarith
-    also have "\<dots> \<le> height l + max(height r) (height l) + 2"
+    also have "\<dots> \<le> height l + max(height r) (height l) + 1"
       using 1 by linarith
-    also have "\<dots> \<le> 2 * (max(height r) (height l) + 1)"
+    also have "\<dots> \<le> 2 * max(height r) (height l) + 1"
       by simp
-    also have "\<dots> \<le> 2 * height t + 1"
+    also have "\<dots> \<le> 2 * height t"
       by simp
     finally show ?thesis .
   qed
